.

pure/UntypedLambdaCalculus.v
@@ -15,6 +15,8 @@ Module UntypedLamdbdaCalculus.
 
   Import ListNotations EqFacts MyUtilities BasicSetoidTheory MyEnsemble BasicPosetTheory BasicTopology.
 
+  Section UNTYPED_LAMBDA_CALCULUS_WITH_CONSTANT.
+
   Definition ivar : Set :=
     nat
   .
@@ -24,146 +26,22 @@ Module UntypedLamdbdaCalculus.
     forall y : ivar,
     {x = y} + {x <> y}.
   Proof.
-    exact Nat.eq_dec.
+    exact (fun x y => Nat.eq_dec x y).
   Defined.
+
+  Variable CON : Set.
 
   Inductive tm : Set :=
   | tmVar : forall x : ivar, tm
+  | tmCon : forall c : CON, tm
   | tmApp : forall P1 : tm, forall P2 : tm, tm
   | tmLam : forall y : ivar, forall Q : tm, tm
   .
 
-  Definition tm_eq_dec :
-    forall M1 : tm,
-    forall M2 : tm,
-    {M1 = M2} + {M1 <> M2}.
-  Proof with try ((left; congruence) || (right; congruence)).
-    induction M1; destruct M2...
-    - destruct (ivar_eq_dec x x0)...
-    - destruct (IHM1_1 M2_1); destruct (IHM1_2 M2_2)...
-    - destruct (ivar_eq_dec y y0); destruct (IHM1 M2)...
-  Defined.
-
-  Section SUBTERM.
-
-  Fixpoint getRank (M : tm) {struct M} : nat :=
-    match M with
-    | tmVar x => 0
-    | tmApp P1 P2 => S (max (getRank P1) (getRank P2))
-    | tmLam y Q => S (getRank Q)
-    end
-  .
-
-  Inductive subtm : tm -> tm -> Set :=
-  | subtmRefl : forall M : tm, subtm M M
-  | subtmAppL : forall M : tm, forall P1 : tm, forall P2 : tm, subtm M P1 -> subtm M (tmApp P1 P2)
-  | subtmAppR : forall M : tm, forall P1 : tm, forall P2 : tm, subtm M P2 -> subtm M (tmApp P1 P2)
-  | subtmLAbs : forall M : tm, forall y : ivar, forall Q : tm, subtm M Q -> subtm M (tmLam y Q)
-  .
-
-  Local Hint Constructors subtm : core.
-
-  Lemma subtm_getRank :
-    forall M : tm,
-    forall N : tm,
-    subtm M N ->
-    getRank M <= getRank N.
-  Proof with lia.
-    intros M N X.
-    induction X; simpl...
-  Qed.
-
-  Lemma subtm_and_same_rank_implies_same_term :
-    forall M : tm,
-    forall N : tm,
-    subtm M N ->
-    getRank M = getRank N ->
-    M = N.
-  Proof with lia.
-    intros M N X.
-    destruct X; simpl; intros H.
-    - reflexivity.
-    - assert (H0 := subtm_getRank M P1 X)...
-    - assert (H0 := subtm_getRank M P2 X)...
-    - assert (H0 := subtm_getRank M Q X)...
-  Qed.
-
-  Lemma subtm_refl :
-    forall M1 : tm,
-    subtm M1 M1.
-  Proof.
-    exact subtmRefl.
-  Qed.
-
-  Lemma subtm_asym :
-    forall M1 : tm,
-    forall M2 : tm,
-    subtm M1 M2 ->
-    subtm M2 M1 ->
-    M1 = M2.
-  Proof with eauto.
-    intros M1 M2 H H0.
-    apply subtm_and_same_rank_implies_same_term...
-    enough (getRank M1 <= getRank M2 /\ getRank M2 <= getRank M1) by lia.
-    split; apply subtm_getRank...
-  Qed.
-
-  Lemma subtm_trans :
-    forall M1 : tm,
-    forall M2 : tm,
-    forall M3 : tm,
-    subtm M1 M2 ->
-    subtm M2 M3 ->
-    subtm M1 M3.
-  Proof with eauto.
-    enough (claim1 : forall L : tm, forall N : tm, forall M : tm, subtm N L -> subtm M N -> subtm M L) by firstorder.
-    induction L; intros N M H H0; inversion H; subst...
-  Qed.
-
-  Local Hint Resolve subtm_refl subtm_asym subtm_trans : core.
-
-  Theorem strong_induction_on_tm (phi : tm -> Prop) :
-    (forall M : tm, (forall N : tm, subtm N M -> N <> M -> phi N) -> phi M) ->
-    forall M : tm,
-    phi M.
-  Proof with (congruence || eauto).
-    intros XXX.
-    enough (claim1 : forall M : tm, forall L : tm, subtm L M -> phi L)...
-    induction M; intros L H; apply XXX; intros N H0 H1; inversion H0; subst...
-    all: inversion H; subst...
-  Qed.
-
-  Definition rect_subtm (L : tm) :
-    forall XP : forall M : tm, subtm L M -> Type,
-    (XP L (subtmRefl L)) ->
-    (forall P1 : tm, forall P2 : tm, forall X : subtm L P1, XP P1 X -> XP (tmApp P1 P2) (subtmAppL L P1 P2 X)) ->
-    (forall P1 : tm, forall P2 : tm, forall X : subtm L P2, XP P2 X -> XP (tmApp P1 P2) (subtmAppR L P1 P2 X)) ->
-    (forall y : ivar, forall Q : tm, forall X : subtm L Q, XP Q X -> XP (tmLam y Q) (subtmLAbs L y Q X)) ->
-    (forall M : tm, forall X : subtm L M, XP M X).
-  Proof.
-    set (my_eq_elim := fun L0 : tm => fun H : L0 = L => fun phi : forall L1 : tm, L1 = L -> Type => fun phi_pf : phi L (eq_reflexivity L) => @rect_eq_r tm L phi phi_pf L0 H).
-    intros XP case_Refl case_AppL case_AppR case_LAbs.
-    set (XP_Refl := fun M0 : tm => fun H : M0 = L => my_eq_elim M0 H (fun M1 : tm => fun H0 : M1 = L => XP M1 (eq_rect M1 (fun N1 : tm => subtm N1 M1) (subtmRefl M1) L H0)) case_Refl).
-    set (XP_AppL := fun M0 : tm => fun P1 : tm => fun P2 : tm => fun H : M0 = L => my_eq_elim M0 H (fun M1 : tm => fun H0 : M1 = L => forall X' : subtm M1 P1, (forall H' : M1 = L, XP P1 (eq_rect M1 (fun N1 : tm => subtm N1 P1) X' L H')) -> XP (tmApp P1 P2) (eq_rect M1 (fun N1 : tm => subtm N1 (tmApp P1 P2)) (subtmAppL M1 P1 P2 X') L H0)) (fun X' : subtm L P1 => fun IHX' : forall H' : L = L, XP P1 (eq_rect L (fun N1 : tm => subtm N1 P1) X' L H') => case_AppL P1 P2 X' (IHX' (eq_reflexivity L)))).
-    set (XP_AppR := fun M0 : tm => fun P1 : tm => fun P2 : tm => fun H : M0 = L => my_eq_elim M0 H (fun M1 : tm => fun H0 : M1 = L => forall X' : subtm M1 P2, (forall H' : M1 = L, XP P2 (eq_rect M1 (fun N1 : tm => subtm N1 P2) X' L H')) -> XP (tmApp P1 P2) (eq_rect M1 (fun N1 : tm => subtm N1 (tmApp P1 P2)) (subtmAppR M1 P1 P2 X') L H0)) (fun X' : subtm L P2 => fun IHX' : forall H' : L = L, XP P2 (eq_rect L (fun N1 : tm => subtm N1 P2) X' L H') => case_AppR P1 P2 X' (IHX' (eq_reflexivity L)))).
-    set (XP_LAbs := fun M0 : tm => fun y : ivar => fun Q : tm => fun H : M0 = L => my_eq_elim M0 H (fun M1 : tm => fun H0 : M1 = L => forall X' : subtm M1 Q, (forall H' : M1 = L, XP Q (eq_rect M1 (fun N1 : tm => subtm N1 Q) X' L H')) -> XP (tmLam y Q) (eq_rect M1 (fun N1 : tm => subtm N1 (tmLam y Q)) (subtmLAbs M1 y Q X') L H0)) (fun X' : subtm L Q => fun IHX' : forall H' : L = L, XP Q (eq_rect L (fun N1 : tm => subtm N1 Q) X' L H') => case_LAbs y Q X' (IHX' (eq_reflexivity L)))).
-    enough (go : forall N : tm, forall M : tm, forall X : subtm N M, forall H : N = L, XP M (eq_rect N (fun N0 : tm => subtm N0 M) X L H)) by exact (fun M : tm => fun X : subtm L M => go L M X (eq_reflexivity L)).
-    exact (
-      fix rect_subtm_fix (N : tm) (M : tm) (X : subtm N M) {struct X} : forall H : N = L, XP M (eq_rect N (fun N1 : tm => subtm N1 M) X L H) :=
-      match X as X0 in subtm N0 M0 return forall H : N0 = L, XP M0 (eq_rect N0 (fun N1 : tm => subtm N1 M0) X0 L H) with
-      | subtmRefl M0 => fun H : M0 = L => XP_Refl M0 H 
-      | subtmAppL M0 P1 P2 X' => fun H : M0 = L => XP_AppL M0 P1 P2 H X' (rect_subtm_fix M0 P1 X')
-      | subtmAppR M0 P1 P2 X' => fun H : M0 = L => XP_AppR M0 P1 P2 H X' (rect_subtm_fix M0 P2 X')
-      | subtmLAbs M0 y Q X' => fun H : M0 = L => XP_LAbs M0 y Q H X' (rect_subtm_fix M0 Q X')
-      end
-    ).
-  Defined.
-
-  End SUBTERM.
-
-  Fixpoint getFVs (M : tm) : list ivar :=
+  Fixpoint getFVs (M : tm) {struct M} : list ivar :=
     match M with
     | tmVar x => [x]
+    | tmCon c => []
     | tmApp P1 P2 => getFVs P1 ++ getFVs P2
     | tmLam y Q => remove ivar_eq_dec y (getFVs Q)
     end
@@ -172,6 +50,7 @@ Module UntypedLamdbdaCalculus.
   Fixpoint isFreeIn (z : ivar) (M : tm) {struct M} : bool :=
     match M with
     | tmVar x => Nat.eqb x z
+    | tmCon c => false
     | tmApp P1 P2 => isFreeIn z P1 || isFreeIn z P2
     | tmLam y Q => isFreeIn z Q && negb (Nat.eqb z y)
     end
@@ -186,28 +65,28 @@ Module UntypedLamdbdaCalculus.
 
   Section SUBSTITUTION. (* Reference: "https://github.com/ernius/formalmetatheory-stoughton/tree/7eea5b526ec58a49838daa7b21b02fafcbf9065e" *)
 
-  Definition substitution : Set :=
+  Definition tmSubst : Set :=
     ivar -> tm
   .
 
-  Definition nil_subtitution : substitution :=
+  Definition tmSubst_nil : tmSubst :=
     tmVar
   .
 
-  Definition cons_substitution : ivar -> tm -> substitution -> substitution :=
+  Definition tmSubst_cons : ivar -> tm -> tmSubst -> tmSubst :=
     fun x : ivar =>
     fun M : tm =>
-    fun sigma : substitution =>
+    fun sigma : tmSubst =>
     fun y : ivar =>
     if ivar_eq_dec x y
     then M
     else sigma y
   .
 
-  Fixpoint mk_substitution (sigma : list (ivar * tm)) {struct sigma} : substitution :=
+  Fixpoint tmSubstMaker (sigma : list (ivar * tm)) {struct sigma} : tmSubst :=
     match sigma with
-    | [] => nil_subtitution
-    | (x, M) :: sigma' => cons_substitution x M (mk_substitution sigma')
+    | [] => tmSubst_nil
+    | (x, M) :: sigma' => tmSubst_cons x M (tmSubstMaker sigma')
     end
   .
 
@@ -227,26 +106,26 @@ Module UntypedLamdbdaCalculus.
     enough (fold_right_max_0 (getFVs M) >= x -> fold_right_max_0 (getFVs M) < x -> False) by eauto...
   Qed.
 
-  Definition isFreshIn_substitution : ivar -> substitution -> tm -> bool :=
+  Definition isFreshIn_tmSubst : ivar -> tmSubst -> tm -> bool :=
     fun x : ivar =>
-    fun sigma : substitution =>
+    fun sigma : tmSubst =>
     fun M : tm =>
     forallb (fun z : ivar => negb (isFreeIn x (sigma z))) (getFVs M)
   .
 
-  Definition chi : substitution -> tm -> ivar :=
-    fun sigma : substitution => 
+  Definition chi : tmSubst -> tm -> ivar :=
+    fun sigma : tmSubst => 
     fun M : tm =>
     S (fold_right_max_0 (map (fun x : ivar => get_max_ivar (sigma x)) (getFVs M)))
   .
 
   Theorem main_property_of_chi :
     forall M : tm,
-    forall sigma : substitution,
-    isFreshIn_substitution (chi sigma M) sigma M = true.
+    forall sigma : tmSubst,
+    isFreshIn_tmSubst (chi sigma M) sigma M = true.
   Proof with auto_rewrite.
     assert ( claim1 :
-      forall sigma : substitution,
+      forall sigma : tmSubst,
       forall M : tm,
       forall x : ivar,
       isFreeIn x M = true ->
@@ -259,60 +138,61 @@ Module UntypedLamdbdaCalculus.
       rewrite <- getFVs_isFreeIn in H.
       apply fold_right_max_0_in...
     }
-    unfold isFreshIn_substitution...
+    unfold isFreshIn_tmSubst...
     apply claim1, getFVs_isFreeIn...
   Qed.
 
   Lemma chi_nil : 
     forall M : tm,
-    isFreeIn (chi nil_subtitution M) M = false.
+    isFreeIn (chi tmSubst_nil M) M = false.
   Proof with auto_rewrite.
     intros M.
-    assert (H : isFreshIn_substitution (chi nil_subtitution M) nil_subtitution M = true) by apply main_property_of_chi.
-    unfold isFreshIn_substitution in H.
+    assert (H : isFreshIn_tmSubst (chi tmSubst_nil M) tmSubst_nil M = true) by apply main_property_of_chi.
+    unfold isFreshIn_tmSubst in H.
     rewrite forallb_true_iff in H.
     simpl in H.
     apply not_true_iff_false.
     intros H0.
-    assert (H1 : negb (chi nil_subtitution M =? chi nil_subtitution M) = true) by now apply H, getFVs_isFreeIn...
+    assert (H1 : negb (chi tmSubst_nil M =? chi tmSubst_nil M) = true) by now apply H, getFVs_isFreeIn...
   Qed.
 
-  Fixpoint run_substitution_on_tm (sigma : substitution) (M : tm) {struct M} : tm :=
+  Fixpoint run_tmSubst_on_tm (sigma : tmSubst) (M : tm) {struct M} : tm :=
     match M with
     | tmVar x => sigma x
-    | tmApp P1 P2 => tmApp (run_substitution_on_tm sigma P1) (run_substitution_on_tm sigma P2)
+    | tmCon c => tmCon c
+    | tmApp P1 P2 => tmApp (run_tmSubst_on_tm sigma P1) (run_tmSubst_on_tm sigma P2)
     | tmLam y Q =>
       let z : ivar := chi sigma M in
-      tmLam z (run_substitution_on_tm (cons_substitution y (tmVar z) sigma) Q)
+      tmLam z (run_tmSubst_on_tm (tmSubst_cons y (tmVar z) sigma) Q)
     end
   .
 
-  Theorem main_property_isFreshIn_substitution :
+  Theorem main_property_isFreshIn_tmSubst :
     forall M : tm,
     forall z : ivar,
-    forall sigma : substitution,
-    isFreshIn_substitution z sigma M = true <-> isFreeIn z (run_substitution_on_tm sigma M) = false.
+    forall sigma : tmSubst,
+    isFreshIn_tmSubst z sigma M = true <-> isFreeIn z (run_tmSubst_on_tm sigma M) = false.
   Proof with auto_rewrite.
-    induction M; unfold isFreshIn_substitution; simpl...
+    induction M; unfold isFreshIn_tmSubst; simpl...
     split; intros H.
     - destruct (ivar_eq_dec z (chi sigma (tmLam y M)))...
       left.
       apply IHM.
-      unfold isFreshIn_substitution, cons_substitution.
+      unfold isFreshIn_tmSubst, tmSubst_cons.
       apply forallb_true_iff.
       intros x H0.
       destruct (ivar_eq_dec y x); [apply negb_true_iff, Nat.eqb_neq | apply H, in_in_remove]...
     - auto_rewrite.
       destruct H0 as [H0 H1].
       destruct H as [H | H].
-      + assert (H2 : isFreshIn_substitution z (cons_substitution y (tmVar (chi sigma (tmLam y M))) sigma) M = true) by now apply IHM.
-        unfold isFreshIn_substitution in H2.
+      + assert (H2 : isFreshIn_tmSubst z (tmSubst_cons y (tmVar (chi sigma (tmLam y M))) sigma) M = true) by now apply IHM.
+        unfold isFreshIn_tmSubst in H2.
         rewrite forallb_true_iff in H2.
         assert (H3 := H2 x H0).
-        unfold cons_substitution in H3.
+        unfold tmSubst_cons in H3.
         destruct (ivar_eq_dec y x)...
-      + assert (H2 : isFreshIn_substitution z sigma (tmLam y M) = true) by now rewrite H; apply main_property_of_chi.
-        unfold isFreshIn_substitution in H2.
+      + assert (H2 : isFreshIn_tmSubst z sigma (tmLam y M) = true) by now rewrite H; apply main_property_of_chi.
+        unfold isFreshIn_tmSubst in H2.
         rewrite forallb_true_iff in H2.
         apply negb_true_iff, H2.
         rewrite getFVs_isFreeIn.
@@ -320,30 +200,30 @@ Module UntypedLamdbdaCalculus.
         rewrite <- getFVs_isFreeIn...
   Qed.
 
-  Definition equiv_substitution_wrt : substitution -> substitution -> tm -> Prop :=
-    fun sigma1 : substitution =>
-    fun sigma2 : substitution =>
+  Definition equiv_tmSubst_wrt : tmSubst -> tmSubst -> tm -> Prop :=
+    fun sigma1 : tmSubst =>
+    fun sigma2 : tmSubst =>
     fun M : tm =>
     forall x : ivar,
     isFreeIn x M = true ->
     sigma1 x = sigma2 x
   .
 
-  Lemma property1_of_equiv_substitution_wrt :
-    forall sigma1 : substitution,
-    forall sigma2 : substitution,
+  Lemma property1_of_equiv_tmSubst_wrt :
+    forall sigma1 : tmSubst,
+    forall sigma2 : tmSubst,
     (forall x : ivar, sigma1 x = sigma2 x) ->
     forall M : tm,
-    equiv_substitution_wrt sigma1 sigma2 M.
+    equiv_tmSubst_wrt sigma1 sigma2 M.
   Proof with try now firstorder.
-    unfold equiv_substitution_wrt...
+    unfold equiv_tmSubst_wrt...
   Qed.
 
-  Lemma chi_equiv_substitution_wrt :
-    forall sigma1 : substitution,
-    forall sigma2 : substitution,
+  Lemma chi_equiv_tmSubst_wrt :
+    forall sigma1 : tmSubst,
+    forall sigma2 : tmSubst,
     forall M : tm,
-    equiv_substitution_wrt sigma1 sigma2 M ->
+    equiv_tmSubst_wrt sigma1 sigma2 M ->
     chi sigma1 M = chi sigma2 M.
   Proof with auto_rewrite.
     unfold chi.
@@ -354,109 +234,110 @@ Module UntypedLamdbdaCalculus.
     rewrite (H x (proj1 (getFVs_isFreeIn M x) H0))...
   Qed.
 
-  Theorem main_property_of_equiv_substitution_wrt :
+  Theorem main_property_of_equiv_tmSubst_wrt :
     forall M : tm,
-    forall sigma1 : substitution,
-    forall sigma2 : substitution,
-    equiv_substitution_wrt sigma1 sigma2 M ->
-    run_substitution_on_tm sigma1 M = run_substitution_on_tm sigma2 M.
+    forall sigma1 : tmSubst,
+    forall sigma2 : tmSubst,
+    equiv_tmSubst_wrt sigma1 sigma2 M ->
+    run_tmSubst_on_tm sigma1 M = run_tmSubst_on_tm sigma2 M.
   Proof with auto_rewrite.
     induction M; simpl.
     - intros sigma1 sigma2 H.
       apply H...
+    - reflexivity.
     - intros sigma1 sigma2 H.
-      enough (claim1 : equiv_substitution_wrt sigma1 sigma2 M1).
-      enough (claim2 : equiv_substitution_wrt sigma1 sigma2 M2).
+      enough (claim1 : equiv_tmSubst_wrt sigma1 sigma2 M1).
+      enough (claim2 : equiv_tmSubst_wrt sigma1 sigma2 M2).
       rewrite (IHM1 sigma1 sigma2 claim1), (IHM2 sigma1 sigma2 claim2)...
       all: intros x H0; apply H...
     - intros sigma1 sigma2 H.
-      enough (claim3 : equiv_substitution_wrt (cons_substitution y (tmVar (chi sigma1 (tmLam y M))) sigma1) (cons_substitution y (tmVar (chi sigma2 (tmLam y M))) sigma2) M).
-      assert (claim4 : chi sigma1 (tmLam y M) = chi sigma2 (tmLam y M)) by now apply chi_equiv_substitution_wrt.
-      rewrite (IHM (cons_substitution y (tmVar (chi sigma1 (tmLam y M))) sigma1) (cons_substitution y (tmVar (chi sigma2 (tmLam y M))) sigma2) claim3), claim4...
+      enough (claim3 : equiv_tmSubst_wrt (tmSubst_cons y (tmVar (chi sigma1 (tmLam y M))) sigma1) (tmSubst_cons y (tmVar (chi sigma2 (tmLam y M))) sigma2) M).
+      assert (claim4 : chi sigma1 (tmLam y M) = chi sigma2 (tmLam y M)) by now apply chi_equiv_tmSubst_wrt.
+      rewrite (IHM (tmSubst_cons y (tmVar (chi sigma1 (tmLam y M))) sigma1) (tmSubst_cons y (tmVar (chi sigma2 (tmLam y M))) sigma2) claim3), claim4...
       intros x H0.
-      unfold cons_substitution.
+      unfold tmSubst_cons.
       destruct (ivar_eq_dec y x).
-      + rewrite (chi_equiv_substitution_wrt sigma1 sigma2 (tmLam y M) H)...
+      + rewrite (chi_equiv_tmSubst_wrt sigma1 sigma2 (tmLam y M) H)...
       + apply H...
   Qed.
 
-  Lemma trivial_substitution :
+  Lemma trivial_tmSubst :
     forall x : ivar,
     forall M : tm,
-    run_substitution_on_tm (cons_substitution x (tmVar x) nil_subtitution) M = run_substitution_on_tm nil_subtitution M.
+    run_tmSubst_on_tm (tmSubst_cons x (tmVar x) tmSubst_nil) M = run_tmSubst_on_tm tmSubst_nil M.
   Proof with try now firstorder.
-    unfold cons_substitution.
+    unfold tmSubst_cons.
     intros x M.
-    apply main_property_of_equiv_substitution_wrt.
+    apply main_property_of_equiv_tmSubst_wrt.
     intros y H.
     destruct (ivar_eq_dec x y)...
   Qed.
 
-  Definition compose_substitution : substitution -> substitution -> substitution :=
-    fun sigma2 : substitution =>
-    fun sigma1 : substitution =>
+  Definition compose_tmSubst : tmSubst -> tmSubst -> tmSubst :=
+    fun sigma2 : tmSubst =>
+    fun sigma1 : tmSubst =>
     fun x : ivar =>
-    run_substitution_on_tm sigma2 (sigma1 x)
+    run_tmSubst_on_tm sigma2 (sigma1 x)
   .
 
   Lemma distri_compose_cons :
     forall M : tm,
     forall N : tm,
-    forall sigma1 : substitution,
-    forall sigma2 : substitution,
+    forall sigma1 : tmSubst,
+    forall sigma2 : tmSubst,
     forall x : ivar,
     forall y : ivar,
-    isFreshIn_substitution y sigma1 (tmLam x M) = true ->
+    isFreshIn_tmSubst y sigma1 (tmLam x M) = true ->
     forall z : ivar,
     isFreeIn z M = true ->
-    cons_substitution x N (compose_substitution sigma2 sigma1) z = compose_substitution (cons_substitution y N sigma2) (cons_substitution x (tmVar y) sigma1) z.
+    tmSubst_cons x N (compose_tmSubst sigma2 sigma1) z = compose_tmSubst (tmSubst_cons y N sigma2) (tmSubst_cons x (tmVar y) sigma1) z.
   Proof with try now firstorder.
     intros M N sigma1 sigma2 x y H z H0.
-    unfold cons_substitution, compose_substitution.
+    unfold tmSubst_cons, compose_tmSubst.
     destruct (ivar_eq_dec x z).
     - simpl.
       destruct (ivar_eq_dec y y)...
-    - unfold isFreshIn_substitution in H.
+    - unfold isFreshIn_tmSubst in H.
       rewrite forallb_true_iff in H.
       assert (claim1 : isFreeIn y (sigma1 z) = false) by now apply negb_true_iff, H, getFVs_isFreeIn; auto_rewrite.
       assert ( claim2 :
         forall u : ivar,
         isFreeIn u (sigma1 z) = true ->
-        cons_substitution y N sigma2 u = sigma2 u
+        tmSubst_cons y N sigma2 u = sigma2 u
       ).
-      { unfold cons_substitution.
+      { unfold tmSubst_cons.
         intros u H1.
         destruct (ivar_eq_dec y u); subst...
         rewrite claim1 in H1...
       }
-      apply main_property_of_equiv_substitution_wrt...
+      apply main_property_of_equiv_tmSubst_wrt...
   Qed.
 
   Corollary distri_compose_cons_for_chi :
     forall M : tm,
     forall N : tm,
-    forall sigma1 : substitution,
-    forall sigma2 : substitution,
+    forall sigma1 : tmSubst,
+    forall sigma2 : tmSubst,
     forall x : ivar,
     let y : ivar := chi sigma1 (tmLam x M) in
     forall z : ivar,
     isFreeIn z M = true ->
-    cons_substitution x N (compose_substitution sigma2 sigma1) z = compose_substitution (cons_substitution y N sigma2) (cons_substitution x (tmVar y) sigma1) z.
+    tmSubst_cons x N (compose_tmSubst sigma2 sigma1) z = compose_tmSubst (tmSubst_cons y N sigma2) (tmSubst_cons x (tmVar y) sigma1) z.
   Proof with eauto using distri_compose_cons, main_property_of_chi.
     intros M N sigma1 sigma2 x y z H...
   Qed.
 
-  Definition FreeIn_wrt : ivar -> substitution -> tm -> Prop :=
+  Definition FreeIn_wrt : ivar -> tmSubst -> tm -> Prop :=
     fun x : ivar =>
-    fun sigma : substitution =>
+    fun sigma : tmSubst =>
     fun M : tm =>
     exists y : ivar, isFreeIn y M = true /\ isFreeIn x (sigma y) = true
   .
 
   Theorem isFreeIn_wrt_true_iff (M : tm) :
     forall z : ivar,
-    forall sigma : substitution,
-    isFreeIn z (run_substitution_on_tm sigma M) = true <-> FreeIn_wrt z sigma M.
+    forall sigma : tmSubst,
+    isFreeIn z (run_tmSubst_on_tm sigma M) = true <-> FreeIn_wrt z sigma M.
   Proof with auto_rewrite.
     unfold FreeIn_wrt.
     induction M; simpl.
@@ -464,6 +345,8 @@ Module UntypedLamdbdaCalculus.
       split; intros H.
       + exists x...
       + destruct H as [y [H H0]]...
+    - firstorder.
+      inversion H.
     - intros z sigma...
       split.
       + intros [H | H]; [assert (it_is_sufficient_to_show : exists y : ivar, isFreeIn y M1 = true /\ isFreeIn z (sigma y) = true) | assert (it_is_sufficient_to_show : exists y : ivar, isFreeIn y M2 = true /\ isFreeIn z (sigma y) = true)]...
@@ -472,26 +355,26 @@ Module UntypedLamdbdaCalculus.
     - intros x sigma...
       split; intros H.
       + destruct H as [H H0].
-        assert (H1 := proj1 (IHM x (cons_substitution y (tmVar (chi sigma (tmLam y M))) sigma)) H).
+        assert (H1 := proj1 (IHM x (tmSubst_cons y (tmVar (chi sigma (tmLam y M))) sigma)) H).
         destruct H1 as [w [H1 H2]].
         set (z := chi sigma (tmLam y M)).
         fold z in H, H0, H2.
         destruct (ivar_eq_dec y w).
         * subst.
-          unfold cons_substitution in H2.
+          unfold tmSubst_cons in H2.
           destruct (ivar_eq_dec w w)...
           unfold isFreeIn in H2.
           rewrite Nat.eqb_eq in H2...
         * exists w...
-          unfold cons_substitution in H2.
+          unfold tmSubst_cons in H2.
           destruct (ivar_eq_dec y w)...
       + rename y into z.
         destruct H as [y [H H0]].
         set (w := chi sigma (tmLam z M))...
         destruct (ivar_eq_dec w x).
         * subst.
-          assert (isFreshIn_substitution w sigma (tmLam z M) = true) by now apply main_property_of_chi.
-          unfold isFreshIn_substitution in H1.
+          assert (isFreshIn_tmSubst w sigma (tmLam z M) = true) by now apply main_property_of_chi.
+          unfold isFreshIn_tmSubst in H1.
           rewrite forallb_true_iff in H1.
           enough (H2 : isFreeIn w (sigma y) = false) by now rewrite H0 in H2.
           apply negb_true_iff, H1, getFVs_isFreeIn...
@@ -499,13 +382,13 @@ Module UntypedLamdbdaCalculus.
           apply IHM.
           exists y.
           split...
-          unfold cons_substitution.
+          unfold tmSubst_cons.
           destruct (ivar_eq_dec z y)...
   Qed.
 
   Lemma chi_ext :
-    forall sigma : substitution,
-    forall sigma' : substitution,
+    forall sigma : tmSubst,
+    forall sigma' : tmSubst,
     forall M : tm,
     forall M' : tm,
     (forall z : ivar, FreeIn_wrt z sigma M <-> FreeIn_wrt z sigma' M') ->
@@ -532,22 +415,22 @@ Module UntypedLamdbdaCalculus.
     rewrite fold_right_max_0_app...
   Qed.
 
-  Theorem main_property_of_compose_substitution :
+  Theorem main_property_of_compose_tmSubst :
     forall M : tm,
-    forall sigma1 : substitution,
-    forall sigma2 : substitution,
-    run_substitution_on_tm sigma2 (run_substitution_on_tm sigma1 M) = run_substitution_on_tm (compose_substitution sigma2 sigma1) M.
+    forall sigma1 : tmSubst,
+    forall sigma2 : tmSubst,
+    run_tmSubst_on_tm sigma2 (run_tmSubst_on_tm sigma1 M) = run_tmSubst_on_tm (compose_tmSubst sigma2 sigma1) M.
   Proof with auto_rewrite.
     induction M; simpl...
     - rewrite IHM1, IHM2...
-    - enough (it_is_sufficient_to_show : chi sigma2 (run_substitution_on_tm sigma1 (tmLam y M)) = chi (compose_substitution sigma2 sigma1) (tmLam y M)).
+    - enough (it_is_sufficient_to_show : chi sigma2 (run_tmSubst_on_tm sigma1 (tmLam y M)) = chi (compose_tmSubst sigma2 sigma1) (tmLam y M)).
       { set (x := chi sigma1 (tmLam y M)).
-        set (x' := chi sigma2 (tmLam x (run_substitution_on_tm (cons_substitution y (tmVar x) sigma1) M))).
-        set (z := chi (compose_substitution sigma2 sigma1) (tmLam y M)).
-        assert (H := IHM (cons_substitution y (tmVar x) sigma1) (cons_substitution x (tmVar x') sigma2)).
+        set (x' := chi sigma2 (tmLam x (run_tmSubst_on_tm (tmSubst_cons y (tmVar x) sigma1) M))).
+        set (z := chi (compose_tmSubst sigma2 sigma1) (tmLam y M)).
+        assert (H := IHM (tmSubst_cons y (tmVar x) sigma1) (tmSubst_cons x (tmVar x') sigma2)).
         rewrite H.
         assert (H0 := distri_compose_cons_for_chi M (tmVar x') sigma1 sigma2 y).
-        assert (H1 : run_substitution_on_tm (compose_substitution (cons_substitution x (tmVar x') sigma2) (cons_substitution y (tmVar x) sigma1)) M = run_substitution_on_tm (cons_substitution y (tmVar x') (compose_substitution sigma2 sigma1)) M) by now apply main_property_of_equiv_substitution_wrt; firstorder.
+        assert (H1 : run_tmSubst_on_tm (compose_tmSubst (tmSubst_cons x (tmVar x') sigma2) (tmSubst_cons y (tmVar x) sigma1)) M = run_tmSubst_on_tm (tmSubst_cons y (tmVar x') (compose_tmSubst sigma2 sigma1)) M) by now apply main_property_of_equiv_tmSubst_wrt; firstorder.
         rewrite H1.
         replace x' with z...
       }
@@ -555,13 +438,13 @@ Module UntypedLamdbdaCalculus.
       set (y := chi sigma1 (tmLam x M)).
       assert ( claim1 :
         forall y' : ivar,
-        (exists x' : ivar, isFreeIn x' (tmLam y (run_substitution_on_tm (cons_substitution x (tmVar y) sigma1) M)) = true /\ isFreeIn y' (sigma2 x') = true) ->
-        (exists u : ivar, isFreeIn u (tmLam x M) = true /\ isFreeIn y' (compose_substitution sigma2 sigma1 u) = true)
+        (exists x' : ivar, isFreeIn x' (tmLam y (run_tmSubst_on_tm (tmSubst_cons x (tmVar y) sigma1) M)) = true /\ isFreeIn y' (sigma2 x') = true) ->
+        (exists u : ivar, isFreeIn u (tmLam x M) = true /\ isFreeIn y' (compose_tmSubst sigma2 sigma1 u) = true)
       ).
       { intros y' [x' [H H0]]...
         destruct H as [H H1].
-        destruct (proj1 (isFreeIn_wrt_true_iff M x' (cons_substitution x (tmVar y) sigma1)) H) as [u [H2 H3]].
-        unfold cons_substitution in H3.
+        destruct (proj1 (isFreeIn_wrt_true_iff M x' (tmSubst_cons x (tmVar y) sigma1)) H) as [u [H2 H3]].
+        unfold tmSubst_cons in H3.
         destruct (ivar_eq_dec x u).
         - unfold isFreeIn in H3.
           rewrite Nat.eqb_eq in H3...
@@ -571,19 +454,19 @@ Module UntypedLamdbdaCalculus.
       }
       assert ( claim2 :
         forall y' : ivar,
-        (exists x' : ivar, isFreeIn x' (tmLam x M) = true /\ isFreeIn y' (compose_substitution sigma2 sigma1 x') = true) ->
-        (exists u : ivar, isFreeIn u (tmLam y (run_substitution_on_tm (cons_substitution x (tmVar y) sigma1) M)) = true /\ isFreeIn y' (sigma2 u) = true)
+        (exists x' : ivar, isFreeIn x' (tmLam x M) = true /\ isFreeIn y' (compose_tmSubst sigma2 sigma1 x') = true) ->
+        (exists u : ivar, isFreeIn u (tmLam y (run_tmSubst_on_tm (tmSubst_cons x (tmVar y) sigma1) M)) = true /\ isFreeIn y' (sigma2 u) = true)
       ).
       { intros y' [x' [H H0]].
         simpl in H.
         rewrite andb_true_iff, negb_true_iff, Nat.eqb_neq in H.
         destruct H as [H H1].
         destruct (proj1 (isFreeIn_wrt_true_iff (sigma1 x') y' sigma2) H0) as [u [H2 H3]].
-        assert (claim2_aux1 : isFreeIn u (run_substitution_on_tm (cons_substitution x (tmVar y) sigma1) M) = true).
+        assert (claim2_aux1 : isFreeIn u (run_tmSubst_on_tm (tmSubst_cons x (tmVar y) sigma1) M) = true).
         { apply isFreeIn_wrt_true_iff.
           exists x'.
           split...
-          unfold cons_substitution.
+          unfold tmSubst_cons.
           destruct (ivar_eq_dec x x')...
         }
         exists u.
@@ -592,7 +475,7 @@ Module UntypedLamdbdaCalculus.
         subst.
         enough (claim2_aux2 : isFreeIn y (sigma1 x') = false) by now rewrite H2 in claim2_aux2.
         assert (H4 := main_property_of_chi (tmLam x M) sigma1).
-        unfold isFreshIn_substitution in H4.
+        unfold isFreshIn_tmSubst in H4.
         rewrite forallb_true_iff in H4.
         apply negb_true_iff, H4.
         rewrite getFVs_isFreeIn...
@@ -603,31 +486,31 @@ Module UntypedLamdbdaCalculus.
   Corollary compose_one :
     forall M : tm,
     forall N : tm,
-    forall sigma : substitution,
+    forall sigma : tmSubst,
     forall x : ivar,
-    run_substitution_on_tm (cons_substitution x (run_substitution_on_tm sigma N) sigma) M = run_substitution_on_tm sigma (run_substitution_on_tm (cons_substitution x N nil_subtitution) M).
+    run_tmSubst_on_tm (tmSubst_cons x (run_tmSubst_on_tm sigma N) sigma) M = run_tmSubst_on_tm sigma (run_tmSubst_on_tm (tmSubst_cons x N tmSubst_nil) M).
   Proof with try now firstorder.
     intros M N sigma x.
-    replace (run_substitution_on_tm (cons_substitution x (run_substitution_on_tm sigma N) sigma) M) with (run_substitution_on_tm (cons_substitution x (run_substitution_on_tm sigma N) (compose_substitution sigma nil_subtitution)) M).
-    replace (run_substitution_on_tm (cons_substitution x (run_substitution_on_tm sigma N) (compose_substitution sigma nil_subtitution)) M) with (run_substitution_on_tm (compose_substitution sigma (cons_substitution x N nil_subtitution)) M).
-    rewrite main_property_of_compose_substitution...
-    all: apply main_property_of_equiv_substitution_wrt, property1_of_equiv_substitution_wrt; unfold compose_substitution, cons_substitution, nil_subtitution; intros z; destruct (ivar_eq_dec x z)...
+    replace (run_tmSubst_on_tm (tmSubst_cons x (run_tmSubst_on_tm sigma N) sigma) M) with (run_tmSubst_on_tm (tmSubst_cons x (run_tmSubst_on_tm sigma N) (compose_tmSubst sigma tmSubst_nil)) M).
+    replace (run_tmSubst_on_tm (tmSubst_cons x (run_tmSubst_on_tm sigma N) (compose_tmSubst sigma tmSubst_nil)) M) with (run_tmSubst_on_tm (compose_tmSubst sigma (tmSubst_cons x N tmSubst_nil)) M).
+    rewrite main_property_of_compose_tmSubst...
+    all: apply main_property_of_equiv_tmSubst_wrt, property1_of_equiv_tmSubst_wrt; unfold compose_tmSubst, tmSubst_cons, tmSubst_nil; intros z; destruct (ivar_eq_dec x z)...
   Qed.
 
-  Theorem main_property_of_cons_substitution :
+  Theorem main_property_of_tmSubst_cons :
     forall x : ivar,
     forall z : ivar,
     forall M : tm,
     forall N : tm,
-    forall sigma : substitution,
+    forall sigma : tmSubst,
     isFreeIn z (tmLam x M) = false ->
-    run_substitution_on_tm (cons_substitution x N sigma) M = run_substitution_on_tm (cons_substitution z N sigma) (run_substitution_on_tm (cons_substitution x (tmVar z) nil_subtitution) M).
+    run_tmSubst_on_tm (tmSubst_cons x N sigma) M = run_tmSubst_on_tm (tmSubst_cons z N sigma) (run_tmSubst_on_tm (tmSubst_cons x (tmVar z) tmSubst_nil) M).
   Proof with auto_rewrite.
     intros x z M N sigma H.
-    rewrite (main_property_of_compose_substitution M (cons_substitution x (tmVar z) nil_subtitution) (cons_substitution z N sigma)).
-    apply main_property_of_equiv_substitution_wrt.
+    rewrite (main_property_of_compose_tmSubst M (tmSubst_cons x (tmVar z) tmSubst_nil) (tmSubst_cons z N sigma)).
+    apply main_property_of_equiv_tmSubst_wrt.
     intros w H0.
-    unfold cons_substitution, nil_subtitution, compose_substitution.
+    unfold tmSubst_cons, tmSubst_nil, compose_tmSubst.
     destruct (ivar_eq_dec x w) as [Heq | Hne]; simpl.
     - destruct (ivar_eq_dec z z)...
     - destruct (ivar_eq_dec z w) as [H_yes | H_no]...
@@ -637,28 +520,21 @@ Module UntypedLamdbdaCalculus.
 
   End SUBSTITUTION.
 
-  Local Notation " M '{'  x '↦' N  '}' " := (run_substitution_on_tm (cons_substitution x N nil_subtitution) M) (at level 10, no associativity).
-
-  Example run_substitution_on_tm_example1 :
-    (tmLam 3 (tmLam 5 (tmApp (tmVar 3) (tmVar 1)))) { 1 ↦ tmApp (tmVar 4) (tmVar 3) } = tmLam 5 (tmLam 6 (tmApp (tmVar 5) (tmApp (tmVar 4) (tmVar 3)))).
-  Proof.
-    reflexivity.
-  Qed.
-
-  Class isPreLambdaStructure (D : Type) `{D_isSetoid : isSetoid D} : Type :=
-    { runApp : D -> arrow D D
-    ; runLam : arrow D D -> D
+  Class isPreLambdaStructure (DOM : Type) `{DOM_isSetoid : isSetoid DOM} : Type :=
+    { runCon : CON -> DOM
+    ; runApp : DOM -> arrow DOM DOM
+    ; runLam : arrow DOM DOM -> DOM
     ; runApp_preserves_eqProp :
-      forall x1 : D,
-      forall y1 : D,
-      forall x2 : D,
-      forall y2 : D,
+      forall x1 : DOM,
+      forall y1 : DOM,
+      forall x2 : DOM,
+      forall y2 : DOM,
       x1 == x2 ->
       y1 == y2 ->
       runApp x1 y1 == runApp x2 y2
     ; runLam_preserves_eqProp :
-      forall f1 : arrow D D,
-      forall f2 : arrow D D,
+      forall f1 : arrow DOM DOM,
+      forall f2 : arrow DOM DOM,
       f1 == f2 ->
       runLam f1 == runLam f2
     }
@@ -668,13 +544,14 @@ Module UntypedLamdbdaCalculus.
 
   Context {D : Type} `{D_isSetoid : isSetoid D} `{D_isPreLambdaStructure : @isPreLambdaStructure D D_isSetoid}.
 
-  Let env : Type :=
+  Let evalEnv : Type :=
     ivar -> D
   .
 
-  Fixpoint eval_tm (E : env) (M : tm) {struct M} : D :=
+  Fixpoint eval_tm (E : evalEnv) (M : tm) {struct M} : D :=
     match M with
     | tmVar x => E x
+    | tmCon c => runCon c
     | tmApp P1 P2 => runApp (eval_tm E P1) (eval_tm E P2)
     | tmLam y Q => runLam (fun v : D => eval_tm (fun z : ivar => if ivar_eq_dec y z then v else E z) Q)
     end
@@ -682,14 +559,15 @@ Module UntypedLamdbdaCalculus.
 
   Lemma eval_tm_ext :
     forall M : tm,
-    forall E1 : env,
-    forall E2 : env,
+    forall E1 : evalEnv,
+    forall E2 : evalEnv,
     (forall z : ivar, isFreeIn z M = true -> E1 z == E2 z) ->
     eval_tm E1 M == eval_tm E2 M.
   Proof with auto_rewrite.
     induction M; simpl.
     - intros E1 E2 H.
       apply H...
+    - reflexivity.
     - intros E1 E2 H.
       apply runApp_preserves_eqProp; [apply IHM1 | apply IHM2]; intros z H0; apply H...
     - intros E1 E2 H.
@@ -701,27 +579,28 @@ Module UntypedLamdbdaCalculus.
 
   Local Hint Resolve eval_tm_ext : core.
 
-  Theorem run_substitution_on_tm_preserves_eval_tm :
+  Theorem run_tmSubst_on_tm_preserves_eval_tm :
     forall M : tm,
-    forall sigma : substitution,
-    forall E : env,
-    eval_tm (fun z : ivar => eval_tm E (sigma z)) M == eval_tm E (run_substitution_on_tm sigma M).
+    forall sigma : tmSubst,
+    forall E : evalEnv,
+    eval_tm (fun z : ivar => eval_tm E (sigma z)) M == eval_tm E (run_tmSubst_on_tm sigma M).
   Proof with eauto with *.
     induction M.
+    - intros sigma E...
     - intros sigma E...
     - intros sigma E.
       apply runApp_preserves_eqProp...
     - intros sigma E.
-      enough (it_is_sufficient_to_show : forall v : D, eval_tm (fun z : ivar => if ivar_eq_dec y z then v else eval_tm E (sigma z)) M == eval_tm (fun z : ivar => if ivar_eq_dec (chi sigma (tmLam y M)) z then v else E z) (run_substitution_on_tm (cons_substitution y (tmVar (chi sigma (tmLam y M))) sigma) M)) by now apply runLam_preserves_eqProp.
+      enough (it_is_sufficient_to_show : forall v : D, eval_tm (fun z : ivar => if ivar_eq_dec y z then v else eval_tm E (sigma z)) M == eval_tm (fun z : ivar => if ivar_eq_dec (chi sigma (tmLam y M)) z then v else E z) (run_tmSubst_on_tm (tmSubst_cons y (tmVar (chi sigma (tmLam y M))) sigma) M)) by now apply runLam_preserves_eqProp.
       intros v.
-      assert (H := IHM (cons_substitution y (tmVar (chi sigma (tmLam y M))) sigma) (fun z : ivar => if ivar_eq_dec (chi sigma (tmLam y M)) z then v else E z)).
+      assert (H := IHM (tmSubst_cons y (tmVar (chi sigma (tmLam y M))) sigma) (fun z : ivar => if ivar_eq_dec (chi sigma (tmLam y M)) z then v else E z)).
       assert ( claim1 :
         forall z : ivar,
         isFreeIn z M = true ->
-        eval_tm (fun x : ivar => if ivar_eq_dec (chi sigma (tmLam y M)) x then v else E x) (cons_substitution y (tmVar (chi sigma (tmLam y M))) sigma z) == (if ivar_eq_dec y z then v else eval_tm E (sigma z))
+        eval_tm (fun x : ivar => if ivar_eq_dec (chi sigma (tmLam y M)) x then v else E x) (tmSubst_cons y (tmVar (chi sigma (tmLam y M))) sigma z) == (if ivar_eq_dec y z then v else eval_tm E (sigma z))
       ).
       { intros z H0.
-        unfold cons_substitution.
+        unfold tmSubst_cons.
         destruct (ivar_eq_dec y z).
         - unfold eval_tm.
           destruct (ivar_eq_dec (chi sigma (tmLam y M)) (chi sigma (tmLam y M)))...
@@ -730,14 +609,14 @@ Module UntypedLamdbdaCalculus.
           intros z' H1.
           destruct (ivar_eq_dec (chi sigma (tmLam y M)) z')...
           subst.
-          assert (H2 : isFreshIn_substitution (chi sigma (tmLam y M)) sigma (tmLam y M) = true) by now apply main_property_of_chi.
-          unfold isFreshIn_substitution in H2.
+          assert (H2 : isFreshIn_tmSubst (chi sigma (tmLam y M)) sigma (tmLam y M) = true) by now apply main_property_of_chi.
+          unfold isFreshIn_tmSubst in H2.
           rewrite forallb_true_iff in H2.
           enough (H3 : isFreeIn (chi sigma (tmLam y M)) (sigma z) = false) by now rewrite H3 in H1.
           apply negb_true_iff, H2, getFVs_isFreeIn.
           auto_rewrite.
       }
-      transitivity (eval_tm (fun z : ivar => eval_tm (fun z0 : ivar => if ivar_eq_dec (chi sigma (tmLam y M)) z0 then v else E z0) (cons_substitution y (tmVar (chi sigma (tmLam y M))) sigma z)) M)...
+      transitivity (eval_tm (fun z : ivar => eval_tm (fun z0 : ivar => if ivar_eq_dec (chi sigma (tmLam y M)) z0 then v else E z0) (tmSubst_cons y (tmVar (chi sigma (tmLam y M))) sigma z)) M)...
   Qed.
 
   End PreliminariesOfSemantics.
@@ -750,156 +629,6 @@ Module UntypedLamdbdaCalculus.
     }
   .
 
-  Section ALPHA_EQUIV_DEFN.
-
-  Let MyType : Type :=
-    Set
-  .
-
-  Inductive DB (vr : MyType) : MyType :=
-  | VarDB : vr -> DB vr
-  | AppDB : DB vr -> DB vr -> DB vr
-  | LamDB : DB vr -> DB vr
-  .
-
-  Definition mkVarDB {vr : MyType} : vr -> DB vr :=
-    VarDB vr
-  .
-
-  Definition mkAppDB {vr : MyType} : DB vr -> DB vr -> DB vr :=
-    AppDB vr
-  .
-
-  Definition mkLamDB {vr : MyType} : DB vr -> DB vr :=
-    LamDB vr
-  .
-
-  Definition fmapDB {A : MyType} {B : MyType} : (A -> B) -> DB A -> DB B :=
-    fun f : A -> B =>
-    fix fmapDB_fix (M : DB A) {struct M} : DB B :=
-    match M with
-    | VarDB _ vr => mkVarDB (f vr)
-    | AppDB _ P1 P2 => mkAppDB (fmapDB_fix P1) (fmapDB_fix P2)
-    | LamDB _ Q => mkLamDB (fmapDB_fix Q)
-    end
-  .
-
-  Fixpoint toDB (ys : list ivar) (M : tm) {struct M} : DB (prod (list ivar) ivar) :=
-    match M with
-    | tmVar x => mkVarDB (ys, x)
-    | tmApp P1 P2 => mkAppDB (toDB ys P1) (toDB ys P2)
-    | tmLam y Q => mkLamDB (toDB (y :: ys) Q)
-    end
-  .
-
-  Let IDX : MyType :=
-    nat
-  .
-
-  Inductive vr : MyType :=
-  | BVAR : IDX -> vr
-  | FVAR : ivar -> vr
-  .
-
-  Definition get_vr : list ivar -> ivar -> vr :=
-    fun ys : list ivar =>
-    fun x : ivar =>
-    maybe (FVAR x) (fun idx : FinSet (length ys) => BVAR (proj1_sig (runFinSet (length ys) idx))) (elemIndex x (ivar_eq_dec x) ys)
-  .
-
-  Let db : MyType :=
-    DB vr
-  .
-
-  Definition mkDeBruijn : tm -> db :=
-    fun M : tm =>
-    fmapDB (fun pr : prod (list ivar) ivar => get_vr (fst pr) (snd pr)) (toDB [] M)
-  .
-
-  Definition alpha : tm -> tm -> Prop :=
-    fun M1 : tm =>
-    fun M2 : tm =>
-    mkDeBruijn M1 = mkDeBruijn M2
-  .
-
-  Local Instance alpha_Equivalence :
-    Equivalence alpha.
-  Proof.
-    split.
-    - intros M1.
-      unfold alpha in *.
-      now reflexivity.
-    - intros M1 M2 Heq1.
-      unfold alpha in *.
-      now symmetry.
-    - intros M1 M2 M3 Heq1 Heq2.
-      unfold alpha in *.
-      now transitivity (mkDeBruijn M2).
-  Qed.
-
-  End ALPHA_EQUIV_DEFN.
-
-  Global Instance tm_isSetoid : isSetoid tm :=
-    { eqProp := alpha
-    ; Setoid_requiresEquivalence := alpha_Equivalence
-    }
-  .
-
-  Section ASSIGN_SIMPLE_TYPE.
-
-  Variable tvar : Set.
-
-  Inductive ty : Set :=
-  | tyVar : forall a : tvar, ty
-  | tyArr : forall tau : ty, forall sigma : ty, ty
-  .
-
-  Local Coercion tyVar : tvar >-> ty.
-
-  Local Notation " tau '→' sigma " := (tyArr tau sigma) (at level 60, right associativity).
-
-  Let tyctx : Set :=
-    list (ivar * ty)
-  .
-
-  Fixpoint lookup_tyctx (x : ivar) (Gamma : tyctx) {struct Gamma} : option ty :=
-    match Gamma with
-    | [] => None
-    | (z, tau) :: Gamma' =>
-      if ivar_eq_dec x z
-      then Some tau
-      else lookup_tyctx x Gamma'
-    end
-  .
-
-  Inductive typing : tyctx -> tm -> ty -> Prop :=
-  | typingVar :
-    forall Gamma : tyctx,
-    forall x : ivar,
-    forall tau : ty,
-    Some tau = lookup_tyctx x Gamma ->
-    typing Gamma (tmVar x) tau
-  | typingApp :
-    forall Gamma : tyctx,
-    forall P1 : tm,
-    forall P2 : tm,
-    forall tau : ty,
-    forall sigma : ty,
-    typing Gamma P1 (tau → sigma) ->
-    typing Gamma P2 tau ->
-    typing Gamma (tmApp P1 P2) sigma
-  | typingLam :
-    forall Gamma : tyctx,
-    forall y : ivar,
-    forall Q : tm,
-    forall tau : ty,
-    forall sigma : ty,
-    typing ((y, tau) :: Gamma) Q sigma ->
-    typing Gamma (tmLam y Q) (tau → sigma)
-  .
-
-  Local Notation " Gamma '⊢' M '\isof' tau " := (typing Gamma M tau) (at level 70, no associativity) : type_scope.
-
-  End ASSIGN_SIMPLE_TYPE.
+  End UNTYPED_LAMBDA_CALCULUS_WITH_CONSTANT.
 
 End UntypedLamdbdaCalculus.
